\begin{tcolorbox}[colback=white]
    \scriptsize
    \begin{align*}
        \Pr[\Phi|_{\mathcal{F}_{h+1}}] & =\sum_{v^0,\ldots,v^h}^{2}\sum_{\vec{o}^0,\ldots,\vec{o}^{h-1}}^{|\vec{O}|}\sum_{s^0,\ldots,s^h}^{|S|}\prod_{t=0}^h\Pr[x_p^t \equiv v^t,x_s^t \equiv s^t,\vec{x_o^t} \equiv \vec{o}^t,x_r^t]\prod_{t=0}^{h-1}\Pr[x_T^t,x_\Omega^t|v^t,s^t,\vec{o}^t]                      \\
                                       & =2^{-(h+1)}\sum_{\hat{t}=1}^{h+1}\sum_{\vec{o}^0,\ldots,\vec{o}^{\hat{t}-2}}^{|\vec{O}|}\sum_{s^0,\ldots,s^{\hat{t}-1}}^{|S|}\prod_{t=0}^{\hat{t}-1}\Pr[x_s^t \equiv s^t,\vec{x_o^t}\equiv\vec{o}^t,x_r^t]\prod_{t=0}^{\hat{t}-2}\Pr[x_T^t,x_\Omega^t|v^t,s^t,\vec{o}^t]  \\
                                       & =2^{-(h+1)}|\vec{O}|^{-h}\sum_{\hat{t}=1}^{h+1}\sum_{\vec{o}^0,\ldots,\vec{o}^{\hat{t}-2}}^{|\vec{O}|}\sum_{s^0,\ldots,s^{\hat{t}-1}}^{|S|}\prod_{t=0}^{\hat{t}-1}\Pr[x_s^t \equiv s^t,x_r^t]\prod_{t=0}^{\hat{t}-2}\Pr[x_T^t,x_\Omega^t|v^t,s^t,\vec{o}^t]               \\
                                       & =2^{-(h+1)}(|\vec{O}|\cdot|S|)^{-h}\sum_{\hat{t}=1}^{h+1}\sum_{\vec{o}^0,\ldots,\vec{o}^{\hat{t}-2}}^{|\vec{O}|}\sum_{s^0,\ldots,s^{\hat{t}-1}}^{|S|}\Pr[x_s^0 \equiv s^0]\prod_{t=0}^{\hat{t}-1}\Pr[x_r^t]\prod_{t=0}^{\hat{t}-2}\Pr[x_T^t,x_\Omega^t|v^t,s^t,\vec{o}^t] \\
                                       & =2^{-(h+1)}(|\vec{O}|\cdot|S|)^{-h}\sum_{\hat{t}=1}^{h+1}\sum_{\vec{o}^0,\ldots,\vec{o}^{\hat{t}-2}}^{|\vec{O}|}\sum_{s^0,\ldots,s^{\hat{t}-1}}^{|S|}\Pr[x_s^0 \equiv s^0]\Pr[x_r^{\hat{t}-1}]\prod_{t=0}^{\hat{t}-2}\Pr[x_T^t,x_\Omega^t|v^t,s^t,\vec{o}^t]              \\
                                       & =\kappa_{h+1}^{-1}\sum_{\hat{t}=1}^{h+1}\sum_{\vec{o}^0,\ldots,\vec{o}^{\hat{t}-2}}^{|\vec{O}|}\sum_{s^0,\ldots,s^{\hat{t}-1}}^{|S|}\Delta_0(s^0)r(s^{\hat{t}-1},\vec{a}^{\hat{t}-1})\prod_{t=0}^{\hat{t}-2}T(s^t,\vec{a}^t,s^{t+1})\Omega(s^{t+1},\vec{a}^t,\vec{o}^t)   \\
                                       & =\kappa_{h+1}^{-1}\sum_{s^0\in S}\Delta_0(s^0)(r(s^0,\vec{a}^0)+\sum_{\vec{o}^0\in \vec{O}}\sum_{s^1\in S}T(s^0,\vec{a}^0,s^1)\Omega(s^1,\vec{a}^0,\vec{o}^0)\Pr[\Phi|_{\mathcal{F}_h}])                                                                                  \\
                                       & =\kappa_{h+1}^{-1}\sum_{s^0\in S}\Delta_0(s^0)(r(s^0,\vec{a}^0)+\sum_{\vec{o}^0\in \vec{O}}\sum_{s^1\in S}T(s^0,\vec{a}^0,s^1)\Omega(s^1,\vec{a}^0,\vec{o}^0)V(\vec{\pi}_h))\text{(induction hypothesis)}                                                                 \\
                                       & =\kappa_{h+1}^{-1} V(\vec{\pi}_{h+1})\text{(by \Cref{eq:dssat-bellman})}
    \end{align*}
\end{tcolorbox}