\begin{tcolorbox}[colback=white]
    \begin{align}
    &\bigwedge_{0\leq t\leq h-2}[x_p^t \equiv \bot\rightarrow\bigwedge_{i\in I}x_o^{i,t} \equiv 0\wedge x_s^{t+1} \equiv 0\wedge x_p^{t+1} \equiv \bot]\label{eq:xp_next}\\
    &x_p^{h-1}\equiv\bot\label{eq:xp_stop}\\
    &\bigwedge_{s\in S}\bigwedge_{\vec{a}\in\vec{A}}[x_p^0 \equiv\bot\wedge x_s^0 \equiv s \wedge\bigwedge_{i\in I}x_a^{i,0}\equiv a_i \rightarrow x_r^0 \equiv N_r(s,\vec{a})]\label{eq:xr_0}\\
    &\bigwedge_{1\leq t\leq h-1}\bigwedge_{s\in S}\bigwedge_{\vec{a}\in\vec{A}}[x_p^{t-1}\equiv\top\wedge x_p^t \equiv\bot\wedge x_s^t \equiv s \wedge\bigwedge_{i\in I}x_a^{i,t}\equiv a_i\rightarrow
    x_r^t \equiv N_r(s,\vec{a})]\label{eq:xr_t}\\
    &\bigwedge_{0\leq t\leq h-2}\bigwedge_{s\in S}\bigwedge_{\vec{a}\in\vec{A}}\bigwedge_{s'\in S}[x_p^t \equiv \top\wedge x_s^t \equiv s \wedge\bigwedge_{i\in I}x_a^{i,t}\equiv a_i\wedge x_s^{t+1}\equiv s'\rightarrow x_{T_{s,\vec{a}}}^t \equiv s']\label{eq:x_T}\\
    &\bigwedge_{0\leq t\leq h-2}\bigwedge_{s'\in S}\bigwedge_{\vec{a}\in\vec{A}}\bigwedge_{\vec{o}\in\vec{O}}[x_p^t \equiv\top\wedge x_s^{t+1} \equiv s'\wedge\bigwedge_{i\in I}x_a^{i,t}\equiv a_i\wedge\bigwedge_{i\in I}x_o^{i,t}\equiv o_i\rightarrow x_{\Omega_{s',\vec{a}}}^t \equiv N_\Omega(\vec{o})]\label{eq:x_omega}
\end{align}
\end{tcolorbox}